\documentclass[12pt, a5paper]{article}

\usepackage[top=1cm,bottom=1cm]{geometry}
\usepackage[utf8]{inputenc}
%\usepackage[spanish]{babel}
\usepackage{amssymb, amsmath, amsbsy}
\usepackage{enumerate}
\usepackage{verbatim}
\usepackage{mathpazo}

\renewcommand{\familydefault}{\sfdefault}

\begin{document}
\subsection*{Arithmetic Properties}
\begin{itemize}
\item{Associative $$a \cdot (b \cdot c) = (a \cdot b) \cdot c$$}
\item{Commutative $$a + b = b + a \quad\text{and}\quad a \cdot b = b \cdot a$$}
\item{Distributive $$a \cdot (b + c) = a \cdot b + a \cdot c$$}
\end{itemize}

\subsubsection*{Arithmetic operations - examples}
\begin{itemize}
\item{$ab + ac = a (b + c)$}
\item{$a\Big(\dfrac{b}{c}\Big) = \dfrac{ab}{c}$}
\item{$\dfrac{(\frac{a}{b})}{c} = \dfrac{a}{bc}$}
\item{$\dfrac{a}{(\frac{b}{c})}= \dfrac{ac}{b}$}
\item{$\dfrac{a}{b} + \dfrac{c}{d} = \dfrac{ad + bc}{bd}$}
\item{$\dfrac{a}{b} - \dfrac{c}{d} = \dfrac{ad - bc}{bd}$}
\item{$\dfrac{a - b}{c - d} = \dfrac{b - a}{d - c}$}
\item{$\dfrac{a + b}{c} = \dfrac{a}{c} + \dfrac{b}{c}$}
\item{$\dfrac{ab + ac}{a} = b + c,\quad a \ne 0$}
\item{$\dfrac{(\frac{a}{b})}{(\frac{c}{d})} = \dfrac{ad}{bc}$}
\end{itemize}

\end{document} 